Marked actors as SDF, removed unnecessary channel invariants

tests/AddDelay.bpl
@@ -19,19 +19,19 @@ const unique this#: Actor;
 // -- End of prelude ---------------------------------------------
 // ---------------------------------------------------------------
 
-procedure Add#anon$0()
+procedure Add#anon$0#0()
   modifies C, R, M, St;
 {
   var i: int;
   var j: int;
   assume true;
 }
-procedure Delay#anon$1()
+procedure Delay#anon$1#1()
   modifies C, R, M, St;
 {
   assume true;
 }
-procedure Delay#anon$2()
+procedure Delay#anon$2#2()
   modifies C, R, M, St;
 {
   var i: int;
@@ -43,7 +43,7 @@ const unique Net#a: Chan (int);
 const unique Net#b: Chan (int);
 const unique Net#c: Chan (int);
 const unique Net#d: Chan (int);
-procedure Net#anon$3#entry()
+procedure Net#anon$3#entry#3()
   modifies C, R, M, St;
 {
   assume C#init[Net#a] == 1;
@@ -66,23 +66,23 @@ procedure Net#anon$3#entry()
   assert {:msg "  Channel invariant might not hold on action entry"} (R[Net#a] + C[Net#a]) == C#init[Net#a];
   assert {:msg "  Channel invariant might not hold on action entry"} 0 <= C[Net#a];
   assert {:msg "  Channel invariant might not hold on action entry"} 0 <= R[Net#a];
-  assert {:msg "  16.15: Channel invariant might not hold on action entry"} (R[Net#c] + C[Net#c]) == R[Net#a];
-  assert {:msg "  17.15: Channel invariant might not hold on action entry"} (R[Net#c] + C[Net#c]) == R[Net#b];
-  assert {:msg "  18.15: Channel invariant might not hold on action entry"} (R[Net#d] + C[Net#d]) == R[Net#a];
-  assert {:msg "  19.15: Channel invariant might not hold on action entry"} (R[Net#d] + C[Net#d]) == R[Net#b];
-  assert {:msg "  20.15: Channel invariant might not hold on action entry"} (R[Net#b] + C[Net#b]) == (R[Net#d] + 1);
-  assert {:msg "  21.16: Channel invariant might not hold on action entry"} (forall i: int :: 
+  assert {:msg "  17.15: Channel invariant might not hold on action entry"} (R[Net#c] + C[Net#c]) == R[Net#a];
+  assert {:msg "  18.15: Channel invariant might not hold on action entry"} (R[Net#c] + C[Net#c]) == R[Net#b];
+  assert {:msg "  19.15: Channel invariant might not hold on action entry"} (R[Net#d] + C[Net#d]) == R[Net#a];
+  assert {:msg "  20.15: Channel invariant might not hold on action entry"} (R[Net#d] + C[Net#d]) == R[Net#b];
+  assert {:msg "  21.15: Channel invariant might not hold on action entry"} (R[Net#b] + C[Net#b]) == (R[Net#d] + 1);
+  assert {:msg "  22.16: Channel invariant might not hold on action entry"} (forall i: int :: 
     (0 <= i) && (i < (R[Net#c] + C[Net#c])) ==> (M[Net#c][i] == (M[Net#a][i] + M[Net#b][i]))
   );
-  assert {:msg "  22.16: Channel invariant might not hold on action entry"} (forall i: int :: 
+  assert {:msg "  23.16: Channel invariant might not hold on action entry"} (forall i: int :: 
     (0 <= i) && (i < (R[Net#d] + C[Net#d])) ==> (M[Net#d][i] == (M[Net#a][i] + M[Net#b][i]))
   );
-  assert {:msg "  23.16: Channel invariant might not hold on action entry"} (forall i: int :: 
+  assert {:msg "  24.16: Channel invariant might not hold on action entry"} (forall i: int :: 
     (1 <= i) && (i < (R[Net#b] + C[Net#b])) ==> (M[Net#b][i] == M[Net#d][i - 1])
   );
-  assert {:msg "  24.15: Channel invariant might not hold on action entry"} M[Net#b][0] == M[Net#c][-1];
+  assert {:msg "  25.15: Channel invariant might not hold on action entry"} M[Net#b][0] == M[Net#c][-1];
 }
-procedure Net#anon$3#Add#anon$0()
+procedure Net#anon$3#Add#anon$0#4()
   modifies C, R, M, St;
 {
   var St#next: State;
@@ -128,37 +128,39 @@ procedure Net#anon$3#Add#anon$0()
   C[Net#c] := C[Net#c] + 1;
   M[Net#d][R[Net#d] + C[Net#d]] := in1#i + in2#j;
   C[Net#d] := C[Net#d] + 1;
-  assert {:msg "  Sub-actor action at 2.3 might not preserve the channel invariant"} 0 <= C[Net#d];
-  assert {:msg "  Sub-actor action at 2.3 might not preserve the channel invariant"} 0 <= R[Net#d];
-  assert {:msg "  Sub-actor action at 2.3 might not preserve the channel invariant"} R[Net#c] == 0;
-  assert {:msg "  Sub-actor action at 2.3 might not preserve the channel invariant"} 0 <= C[Net#c];
-  assert {:msg "  Sub-actor action at 2.3 might not preserve the channel invariant"} 0 <= R[Net#c];
-  assert {:msg "  Sub-actor action at 2.3 might not preserve the channel invariant"} 0 <= C[Net#b];
-  assert {:msg "  Sub-actor action at 2.3 might not preserve the channel invariant"} 0 <= R[Net#b];
-  assert {:msg "  Sub-actor action at 2.3 might not preserve the channel invariant"} (R[Net#a] + C[Net#a]) == C#init[Net#a];
-  assert {:msg "  Sub-actor action at 2.3 might not preserve the channel invariant"} 0 <= C[Net#a];
-  assert {:msg "  Sub-actor action at 2.3 might not preserve the channel invariant"} 0 <= R[Net#a];
-  assert {:msg "  16.15: Sub-actor action at 2.3 might not preserve the channel invariant"} (R[Net#c] + C[Net#c]) == R[Net#a];
-  assert {:msg "  17.15: Sub-actor action at 2.3 might not preserve the channel invariant"} (R[Net#c] + C[Net#c]) == R[Net#b];
-  assert {:msg "  18.15: Sub-actor action at 2.3 might not preserve the channel invariant"} (R[Net#d] + C[Net#d]) == R[Net#a];
-  assert {:msg "  19.15: Sub-actor action at 2.3 might not preserve the channel invariant"} (R[Net#d] + C[Net#d]) == R[Net#b];
-  assert {:msg "  20.15: Sub-actor action at 2.3 might not preserve the channel invariant"} (R[Net#b] + C[Net#b]) == (R[Net#d] + 1);
-  assert {:msg "  21.16: Sub-actor action at 2.3 might not preserve the channel invariant"} (forall i: int :: 
+  assert {:msg "  Sub-actor action at 3.3 might not preserve the channel invariant"} 0 <= C[Net#d];
+  assert {:msg "  Sub-actor action at 3.3 might not preserve the channel invariant"} 0 <= R[Net#d];
+  assert {:msg "  Sub-actor action at 3.3 might not preserve the channel invariant"} R[Net#c] == 0;
+  assert {:msg "  Sub-actor action at 3.3 might not preserve the channel invariant"} 0 <= C[Net#c];
+  assert {:msg "  Sub-actor action at 3.3 might not preserve the channel invariant"} 0 <= R[Net#c];
+  assert {:msg "  Sub-actor action at 3.3 might not preserve the channel invariant"} 0 <= C[Net#b];
+  assert {:msg "  Sub-actor action at 3.3 might not preserve the channel invariant"} 0 <= R[Net#b];
+  assert {:msg "  Sub-actor action at 3.3 might not preserve the channel invariant"} (R[Net#a] + C[Net#a]) == C#init[Net#a];
+  assert {:msg "  Sub-actor action at 3.3 might not preserve the channel invariant"} 0 <= C[Net#a];
+  assert {:msg "  Sub-actor action at 3.3 might not preserve the channel invariant"} 0 <= R[Net#a];
+  assert {:msg "  17.15: Sub-actor action at 3.3 might not preserve the channel invariant"} (R[Net#c] + C[Net#c]) == R[Net#a];
+  assert {:msg "  18.15: Sub-actor action at 3.3 might not preserve the channel invariant"} (R[Net#c] + C[Net#c]) == R[Net#b];
+  assert {:msg "  19.15: Sub-actor action at 3.3 might not preserve the channel invariant"} (R[Net#d] + C[Net#d]) == R[Net#a];
+  assert {:msg "  20.15: Sub-actor action at 3.3 might not preserve the channel invariant"} (R[Net#d] + C[Net#d]) == R[Net#b];
+  assert {:msg "  21.15: Sub-actor action at 3.3 might not preserve the channel invariant"} (R[Net#b] + C[Net#b]) == (R[Net#d] + 1);
+  assert {:msg "  22.16: Sub-actor action at 3.3 might not preserve the channel invariant"} (forall i: int :: 
     (0 <= i) && (i < (R[Net#c] + C[Net#c])) ==> (M[Net#c][i] == (M[Net#a][i] + M[Net#b][i]))
   );
-  assert {:msg "  22.16: Sub-actor action at 2.3 might not preserve the channel invariant"} (forall i: int :: 
+  assert {:msg "  23.16: Sub-actor action at 3.3 might not preserve the channel invariant"} (forall i: int :: 
     (0 <= i) && (i < (R[Net#d] + C[Net#d])) ==> (M[Net#d][i] == (M[Net#a][i] + M[Net#b][i]))
   );
-  assert {:msg "  23.16: Sub-actor action at 2.3 might not preserve the channel invariant"} (forall i: int :: 
+  assert {:msg "  24.16: Sub-actor action at 3.3 might not preserve the channel invariant"} (forall i: int :: 
     (1 <= i) && (i < (R[Net#b] + C[Net#b])) ==> (M[Net#b][i] == M[Net#d][i - 1])
   );
-  assert {:msg "  24.15: Sub-actor action at 2.3 might not preserve the channel invariant"} M[Net#b][0] == M[Net#c][-1];
+  assert {:msg "  25.15: Sub-actor action at 3.3 might not preserve the channel invariant"} M[Net#b][0] == M[Net#c][-1];
 }
-procedure Net#anon$3#Delay#anon$2()
+procedure Net#anon$3#Delay#anon$2#5()
   modifies C, R, M, St;
 {
+  var ActorParam#k: int;
   var St#next: State;
   var in#i: int;
+  assume ActorParam#k == 0;
   assume C#init[Net#a] == 1;
   assume C#init[Net#c] == 0;
   assume C#init[Net#d] == 0;
@@ -194,33 +196,33 @@ procedure Net#anon$3#Delay#anon$2()
   C[Net#d] := C[Net#d] - 1;
   M[Net#b][R[Net#b] + C[Net#b]] := in#i;
   C[Net#b] := C[Net#b] + 1;
-  assert {:msg "  Sub-actor action at 7.3 might not preserve the channel invariant"} 0 <= C[Net#d];
-  assert {:msg "  Sub-actor action at 7.3 might not preserve the channel invariant"} 0 <= R[Net#d];
-  assert {:msg "  Sub-actor action at 7.3 might not preserve the channel invariant"} R[Net#c] == 0;
-  assert {:msg "  Sub-actor action at 7.3 might not preserve the channel invariant"} 0 <= C[Net#c];
-  assert {:msg "  Sub-actor action at 7.3 might not preserve the channel invariant"} 0 <= R[Net#c];
-  assert {:msg "  Sub-actor action at 7.3 might not preserve the channel invariant"} 0 <= C[Net#b];
-  assert {:msg "  Sub-actor action at 7.3 might not preserve the channel invariant"} 0 <= R[Net#b];
-  assert {:msg "  Sub-actor action at 7.3 might not preserve the channel invariant"} (R[Net#a] + C[Net#a]) == C#init[Net#a];
-  assert {:msg "  Sub-actor action at 7.3 might not preserve the channel invariant"} 0 <= C[Net#a];
-  assert {:msg "  Sub-actor action at 7.3 might not preserve the channel invariant"} 0 <= R[Net#a];
-  assert {:msg "  16.15: Sub-actor action at 7.3 might not preserve the channel invariant"} (R[Net#c] + C[Net#c]) == R[Net#a];
-  assert {:msg "  17.15: Sub-actor action at 7.3 might not preserve the channel invariant"} (R[Net#c] + C[Net#c]) == R[Net#b];
-  assert {:msg "  18.15: Sub-actor action at 7.3 might not preserve the channel invariant"} (R[Net#d] + C[Net#d]) == R[Net#a];
-  assert {:msg "  19.15: Sub-actor action at 7.3 might not preserve the channel invariant"} (R[Net#d] + C[Net#d]) == R[Net#b];
-  assert {:msg "  20.15: Sub-actor action at 7.3 might not preserve the channel invariant"} (R[Net#b] + C[Net#b]) == (R[Net#d] + 1);
-  assert {:msg "  21.16: Sub-actor action at 7.3 might not preserve the channel invariant"} (forall i: int :: 
+  assert {:msg "  Sub-actor action at 8.3 might not preserve the channel invariant"} 0 <= C[Net#d];
+  assert {:msg "  Sub-actor action at 8.3 might not preserve the channel invariant"} 0 <= R[Net#d];
+  assert {:msg "  Sub-actor action at 8.3 might not preserve the channel invariant"} R[Net#c] == 0;
+  assert {:msg "  Sub-actor action at 8.3 might not preserve the channel invariant"} 0 <= C[Net#c];
+  assert {:msg "  Sub-actor action at 8.3 might not preserve the channel invariant"} 0 <= R[Net#c];
+  assert {:msg "  Sub-actor action at 8.3 might not preserve the channel invariant"} 0 <= C[Net#b];
+  assert {:msg "  Sub-actor action at 8.3 might not preserve the channel invariant"} 0 <= R[Net#b];
+  assert {:msg "  Sub-actor action at 8.3 might not preserve the channel invariant"} (R[Net#a] + C[Net#a]) == C#init[Net#a];
+  assert {:msg "  Sub-actor action at 8.3 might not preserve the channel invariant"} 0 <= C[Net#a];
+  assert {:msg "  Sub-actor action at 8.3 might not preserve the channel invariant"} 0 <= R[Net#a];
+  assert {:msg "  17.15: Sub-actor action at 8.3 might not preserve the channel invariant"} (R[Net#c] + C[Net#c]) == R[Net#a];
+  assert {:msg "  18.15: Sub-actor action at 8.3 might not preserve the channel invariant"} (R[Net#c] + C[Net#c]) == R[Net#b];
+  assert {:msg "  19.15: Sub-actor action at 8.3 might not preserve the channel invariant"} (R[Net#d] + C[Net#d]) == R[Net#a];
+  assert {:msg "  20.15: Sub-actor action at 8.3 might not preserve the channel invariant"} (R[Net#d] + C[Net#d]) == R[Net#b];
+  assert {:msg "  21.15: Sub-actor action at 8.3 might not preserve the channel invariant"} (R[Net#b] + C[Net#b]) == (R[Net#d] + 1);
+  assert {:msg "  22.16: Sub-actor action at 8.3 might not preserve the channel invariant"} (forall i: int :: 
     (0 <= i) && (i < (R[Net#c] + C[Net#c])) ==> (M[Net#c][i] == (M[Net#a][i] + M[Net#b][i]))
   );
-  assert {:msg "  22.16: Sub-actor action at 7.3 might not preserve the channel invariant"} (forall i: int :: 
+  assert {:msg "  23.16: Sub-actor action at 8.3 might not preserve the channel invariant"} (forall i: int :: 
     (0 <= i) && (i < (R[Net#d] + C[Net#d])) ==> (M[Net#d][i] == (M[Net#a][i] + M[Net#b][i]))
   );
-  assert {:msg "  23.16: Sub-actor action at 7.3 might not preserve the channel invariant"} (forall i: int :: 
+  assert {:msg "  24.16: Sub-actor action at 8.3 might not preserve the channel invariant"} (forall i: int :: 
     (1 <= i) && (i < (R[Net#b] + C[Net#b])) ==> (M[Net#b][i] == M[Net#d][i - 1])
   );
-  assert {:msg "  24.15: Sub-actor action at 7.3 might not preserve the channel invariant"} M[Net#b][0] == M[Net#c][-1];
+  assert {:msg "  25.15: Sub-actor action at 8.3 might not preserve the channel invariant"} M[Net#b][0] == M[Net#c][-1];
 }
-procedure Net#anon$3#exit()
+procedure Net#anon$3#exit#6()
   modifies C, R, M, St;
 {
   assume C#init[Net#a] == 1;
@@ -252,12 +254,12 @@ procedure Net#anon$3#exit()
   );
   assume M[Net#b][0] == M[Net#c][-1];
   assume !(((1 <= C[Net#a]) && (1 <= C[Net#b])) || (1 <= C[Net#d]));
-  assert {:msg "  11.3: The network might leave unread tokens on channel a"} C[Net#a] == 0;
-  assert {:msg "  11.3: The network might not produce the specified number of tokens on output out"} C[Net#c] == 1;
-  assert {:msg "  11.3: The network might leave unread tokens on channel d"} C[Net#d] == 0;
-  assert {:msg "  11.26: Network output might not conform to specified action output"} M[Net#c][0] == (M[Net#c][R[Net#c] - 1] + M[Net#a][0]);
+  assert {:msg "  12.3: The network might leave unread tokens on channel a"} C[Net#a] == 0;
+  assert {:msg "  12.3: The network might not produce the specified number of tokens on output out"} C[Net#c] == 1;
+  assert {:msg "  12.3: The network might leave unread tokens on channel d"} C[Net#d] == 0;
+  assert {:msg "  12.26: Network output might not conform to specified action output"} M[Net#c][0] == (M[Net#c][R[Net#c] - 1] + M[Net#a][0]);
   R[Net#c] := R[Net#c] + C[Net#c];
   C[Net#c] := 0;
-  assert {:msg "  13.13: The network might not preserve the network invariant"} C[Net#b] == 1;
-  assert {:msg "  14.13: The network might not preserve the network invariant"} M[Net#b][R[Net#b]] == M[Net#c][R[Net#c] - 1];
+  assert {:msg "  14.13: The network might not preserve the network invariant"} C[Net#b] == 1;
+  assert {:msg "  15.13: The network might not preserve the network invariant"} M[Net#b][R[Net#b]] == M[Net#c][R[Net#c] - 1];
 }
