tests/DataDependent.bpl
@@ -1,49 +1,58 @@
-
 // ---------------------------------------------------------------
 // -- Types and global variables ---------------------------------
 // ---------------------------------------------------------------
 type Chan a;
+type Actor;
 type CType = <a>[Chan a]int;
 type MType = <a>[Chan a][int]a;
 type State;
+
 var M: MType;
 var C: CType;
 var R: CType; 
 var C#init: CType;
+var St: [Actor]State;
 
-function at$abs(x: int): int { if 0 <= x then x else -x }
-function at$div(int, int): int;
-function at$mod(int, int): int;
-axiom (forall a,b: int :: at$div(a,b)*b + at$mod(a,b) == a);
-axiom (forall a,b: int :: 0 <= at$mod(a,b) && at$mod(a,b) < at$abs(b));
+const unique this#: Actor;
+
+function AT#Abs(x: int): int { if 0 <= x then x else -x }
+function AT#Div(int, int): int;
+function AT#Mod(int, int): int;
+axiom (forall a,b: int :: AT#Div(a,b)*b + AT#Mod(a,b) == a);
+axiom (forall a,b: int :: 0 <= AT#Mod(a,b) && AT#Mod(a,b) < AT#Abs(b));
 
 // ---------------------------------------------------------------
 // -- End of prelude ---------------------------------------------
 // ---------------------------------------------------------------
 
-procedure Repeater#anon$0()
+procedure Repeater#anon$0#0()
+  modifies C, R, M, St;
 {
   var i: int;
   assume true;
 }
-procedure Split#anon$1()
+procedure Split#anon$1#1()
+  modifies C, R, M, St;
 {
   var i: int;
   assume 0 <= i;
   assume true;
 }
-procedure Split#anon$2()
+procedure Split#anon$2#2()
+  modifies C, R, M, St;
 {
   var i: int;
   assume i < 0;
   assume true;
 }
+const unique Net#rep: Actor;
+const unique Net#split: Actor;
 const unique Net#a: Chan (int);
 const unique Net#b: Chan (int);
 const unique Net#c: Chan (int);
 const unique Net#d: Chan (int);
-procedure Net#anon$3#entry()
-  modifies C, R, M;
+procedure Net#anon$3#entry#3()
+  modifies C, R, M, St;
 {
   assume C#init[Net#a] == 2;
   assume C#init[Net#b] == 0;
@@ -55,39 +64,41 @@ procedure Net#anon$3#entry()
   assume R[Net#d] == 0;
   assume (M[Net#a][0] < 0) && (M[Net#a][1] > 0);
   assume C#init == C;
-  assert {:msg "  Channel invariant might not hold on action entry"} R[Net#d] == 0;
-  assert {:msg "  Channel invariant might not hold on action entry"} 0 <= C[Net#d];
-  assert {:msg "  Channel invariant might not hold on action entry"} 0 <= R[Net#d];
-  assert {:msg "  Channel invariant might not hold on action entry"} R[Net#c] == 0;
-  assert {:msg "  Channel invariant might not hold on action entry"} 0 <= C[Net#c];
-  assert {:msg "  Channel invariant might not hold on action entry"} 0 <= R[Net#c];
-  assert {:msg "  Channel invariant might not hold on action entry"} 0 <= C[Net#b];
-  assert {:msg "  Channel invariant might not hold on action entry"} 0 <= R[Net#b];
-  assert {:msg "  Channel invariant might not hold on action entry"} (R[Net#a] + C[Net#a]) == C#init[Net#a];
-  assert {:msg "  Channel invariant might not hold on action entry"} 0 <= C[Net#a];
-  assert {:msg "  Channel invariant might not hold on action entry"} 0 <= R[Net#a];
-  assert {:msg "  19.15: Channel invariant might not hold on action entry"} (M[Net#a][0] < 0) && (M[Net#a][1] > 0);
-  assert {:msg "  20.15: Channel invariant might not hold on action entry"} (R[Net#b] + C[Net#b]) == R[Net#a];
-  assert {:msg "  21.15: Channel invariant might not hold on action entry"} (R[Net#d] + C[Net#d]) == at$div(R[Net#b] + 1, 2);
-  assert {:msg "  22.15: Channel invariant might not hold on action entry"} (R[Net#c] + C[Net#c]) == at$div(R[Net#b], 2);
-  assert {:msg "  23.16: Channel invariant might not hold on action entry"} (forall i: int :: 
+  assert {:msg "  Channel invariant might not hold on action entry (generated)"} R[Net#a] == (R[Net#b] + C[Net#b]);
+  assert {:msg "  Channel invariant might not hold on action entry (generated)"} R[Net#d] == 0;
+  assert {:msg "  Channel invariant might not hold on action entry (generated)"} 0 <= C[Net#d];
+  assert {:msg "  Channel invariant might not hold on action entry (generated)"} 0 <= R[Net#d];
+  assert {:msg "  Channel invariant might not hold on action entry (generated)"} R[Net#c] == 0;
+  assert {:msg "  Channel invariant might not hold on action entry (generated)"} 0 <= C[Net#c];
+  assert {:msg "  Channel invariant might not hold on action entry (generated)"} 0 <= R[Net#c];
+  assert {:msg "  Channel invariant might not hold on action entry (generated)"} 0 <= C[Net#b];
+  assert {:msg "  Channel invariant might not hold on action entry (generated)"} 0 <= R[Net#b];
+  assert {:msg "  Channel invariant might not hold on action entry (generated)"} (R[Net#a] + C[Net#a]) == C#init[Net#a];
+  assert {:msg "  Channel invariant might not hold on action entry (generated)"} 0 <= C[Net#a];
+  assert {:msg "  Channel invariant might not hold on action entry (generated)"} 0 <= R[Net#a];
+  assert {:msg "  20.3: Channel invariant might not hold on action entry"} (M[Net#a][0] < 0) && (M[Net#a][1] > 0);
+  assert {:msg "  21.3: Channel invariant might not hold on action entry"} (R[Net#d] + C[Net#d]) == AT#Div(R[Net#b] + 1, 2);
+  assert {:msg "  22.3: Channel invariant might not hold on action entry"} (R[Net#c] + C[Net#c]) == AT#Div(R[Net#b], 2);
+  assert {:msg "  23.3: Channel invariant might not hold on action entry"} (forall i: int :: 
     (0 <= i) && (i < (R[Net#b] + C[Net#b])) ==> (M[Net#b][i] == M[Net#a][i])
   );
-  assert {:msg "  24.16: Channel invariant might not hold on action entry"} (forall i: int :: 
-    (0 <= i) && (i < R[Net#b]) && (at$mod(i, 2) == 0) ==> (M[Net#b][i] == M[Net#d][at$div(i, 2)])
+  assert {:msg "  24.3: Channel invariant might not hold on action entry"} (forall i: int :: 
+    (0 <= i) && (i < R[Net#b]) && (AT#Mod(i, 2) == 0) ==> (M[Net#b][i] == M[Net#d][AT#Div(i, 2)])
   );
-  assert {:msg "  25.16: Channel invariant might not hold on action entry"} (forall i: int :: 
-    (0 <= i) && (i < R[Net#b]) && (at$mod(i, 2) == 1) ==> (M[Net#b][i] == M[Net#c][at$div(i, 2)])
+  assert {:msg "  25.3: Channel invariant might not hold on action entry"} (forall i: int :: 
+    (0 <= i) && (i < R[Net#b]) && (AT#Mod(i, 2) == 1) ==> (M[Net#b][i] == M[Net#c][AT#Div(i, 2)])
   );
 }
-procedure Net#anon$3#Repeater#anon$0()
-  modifies C, R, M;
+procedure Net#anon$3#Repeater#anon$0#4()
+  modifies C, R, M, St;
 {
+  var St#next: State;
   var in#i: int;
   assume C#init[Net#a] == 2;
   assume C#init[Net#b] == 0;
   assume C#init[Net#c] == 0;
   assume C#init[Net#d] == 0;
+  assume R[Net#a] == (R[Net#b] + C[Net#b]);
   assume R[Net#d] == 0;
   assume 0 <= C[Net#d];
   assume 0 <= R[Net#d];
@@ -100,57 +111,59 @@ procedure Net#anon$3#Repeater#anon$0()
   assume 0 <= C[Net#a];
   assume 0 <= R[Net#a];
   assume (M[Net#a][0] < 0) && (M[Net#a][1] > 0);
-  assume (R[Net#b] + C[Net#b]) == R[Net#a];
-  assume (R[Net#d] + C[Net#d]) == at$div(R[Net#b] + 1, 2);
-  assume (R[Net#c] + C[Net#c]) == at$div(R[Net#b], 2);
+  assume (R[Net#d] + C[Net#d]) == AT#Div(R[Net#b] + 1, 2);
+  assume (R[Net#c] + C[Net#c]) == AT#Div(R[Net#b], 2);
   assume (forall i: int :: 
     (0 <= i) && (i < (R[Net#b] + C[Net#b])) ==> (M[Net#b][i] == M[Net#a][i])
   );
   assume (forall i: int :: 
-    (0 <= i) && (i < R[Net#b]) && (at$mod(i, 2) == 0) ==> (M[Net#b][i] == M[Net#d][at$div(i, 2)])
+    (0 <= i) && (i < R[Net#b]) && (AT#Mod(i, 2) == 0) ==> (M[Net#b][i] == M[Net#d][AT#Div(i, 2)])
   );
   assume (forall i: int :: 
-    (0 <= i) && (i < R[Net#b]) && (at$mod(i, 2) == 1) ==> (M[Net#b][i] == M[Net#c][at$div(i, 2)])
+    (0 <= i) && (i < R[Net#b]) && (AT#Mod(i, 2) == 1) ==> (M[Net#b][i] == M[Net#c][AT#Div(i, 2)])
   );
+  assume true;
   assume 1 <= C[Net#a];
   in#i := M[Net#a][R[Net#a]];
   R[Net#a] := R[Net#a] + 1;
   C[Net#a] := C[Net#a] - 1;
   M[Net#b][R[Net#b] + C[Net#b]] := in#i;
   C[Net#b] := C[Net#b] + 1;
-  assert {:msg "  Sub-actor action at 2.3 might not preserve the channel invariant"} R[Net#d] == 0;
-  assert {:msg "  Sub-actor action at 2.3 might not preserve the channel invariant"} 0 <= C[Net#d];
-  assert {:msg "  Sub-actor action at 2.3 might not preserve the channel invariant"} 0 <= R[Net#d];
-  assert {:msg "  Sub-actor action at 2.3 might not preserve the channel invariant"} R[Net#c] == 0;
-  assert {:msg "  Sub-actor action at 2.3 might not preserve the channel invariant"} 0 <= C[Net#c];
-  assert {:msg "  Sub-actor action at 2.3 might not preserve the channel invariant"} 0 <= R[Net#c];
-  assert {:msg "  Sub-actor action at 2.3 might not preserve the channel invariant"} 0 <= C[Net#b];
-  assert {:msg "  Sub-actor action at 2.3 might not preserve the channel invariant"} 0 <= R[Net#b];
-  assert {:msg "  Sub-actor action at 2.3 might not preserve the channel invariant"} (R[Net#a] + C[Net#a]) == C#init[Net#a];
-  assert {:msg "  Sub-actor action at 2.3 might not preserve the channel invariant"} 0 <= C[Net#a];
-  assert {:msg "  Sub-actor action at 2.3 might not preserve the channel invariant"} 0 <= R[Net#a];
-  assert {:msg "  19.15: Sub-actor action at 2.3 might not preserve the channel invariant"} (M[Net#a][0] < 0) && (M[Net#a][1] > 0);
-  assert {:msg "  20.15: Sub-actor action at 2.3 might not preserve the channel invariant"} (R[Net#b] + C[Net#b]) == R[Net#a];
-  assert {:msg "  21.15: Sub-actor action at 2.3 might not preserve the channel invariant"} (R[Net#d] + C[Net#d]) == at$div(R[Net#b] + 1, 2);
-  assert {:msg "  22.15: Sub-actor action at 2.3 might not preserve the channel invariant"} (R[Net#c] + C[Net#c]) == at$div(R[Net#b], 2);
-  assert {:msg "  23.16: Sub-actor action at 2.3 might not preserve the channel invariant"} (forall i: int :: 
+  assert {:msg "  Sub-actor action at 3.3 might not preserve the channel invariant (generated)"} R[Net#a] == (R[Net#b] + C[Net#b]);
+  assert {:msg "  Sub-actor action at 3.3 might not preserve the channel invariant (generated)"} R[Net#d] == 0;
+  assert {:msg "  Sub-actor action at 3.3 might not preserve the channel invariant (generated)"} 0 <= C[Net#d];
+  assert {:msg "  Sub-actor action at 3.3 might not preserve the channel invariant (generated)"} 0 <= R[Net#d];
+  assert {:msg "  Sub-actor action at 3.3 might not preserve the channel invariant (generated)"} R[Net#c] == 0;
+  assert {:msg "  Sub-actor action at 3.3 might not preserve the channel invariant (generated)"} 0 <= C[Net#c];
+  assert {:msg "  Sub-actor action at 3.3 might not preserve the channel invariant (generated)"} 0 <= R[Net#c];
+  assert {:msg "  Sub-actor action at 3.3 might not preserve the channel invariant (generated)"} 0 <= C[Net#b];
+  assert {:msg "  Sub-actor action at 3.3 might not preserve the channel invariant (generated)"} 0 <= R[Net#b];
+  assert {:msg "  Sub-actor action at 3.3 might not preserve the channel invariant (generated)"} (R[Net#a] + C[Net#a]) == C#init[Net#a];
+  assert {:msg "  Sub-actor action at 3.3 might not preserve the channel invariant (generated)"} 0 <= C[Net#a];
+  assert {:msg "  Sub-actor action at 3.3 might not preserve the channel invariant (generated)"} 0 <= R[Net#a];
+  assert {:msg "  20.3: Sub-actor action at 3.3 might not preserve the channel invariant"} (M[Net#a][0] < 0) && (M[Net#a][1] > 0);
+  assert {:msg "  21.3: Sub-actor action at 3.3 might not preserve the channel invariant"} (R[Net#d] + C[Net#d]) == AT#Div(R[Net#b] + 1, 2);
+  assert {:msg "  22.3: Sub-actor action at 3.3 might not preserve the channel invariant"} (R[Net#c] + C[Net#c]) == AT#Div(R[Net#b], 2);
+  assert {:msg "  23.3: Sub-actor action at 3.3 might not preserve the channel invariant"} (forall i: int :: 
     (0 <= i) && (i < (R[Net#b] + C[Net#b])) ==> (M[Net#b][i] == M[Net#a][i])
   );
-  assert {:msg "  24.16: Sub-actor action at 2.3 might not preserve the channel invariant"} (forall i: int :: 
-    (0 <= i) && (i < R[Net#b]) && (at$mod(i, 2) == 0) ==> (M[Net#b][i] == M[Net#d][at$div(i, 2)])
+  assert {:msg "  24.3: Sub-actor action at 3.3 might not preserve the channel invariant"} (forall i: int :: 
+    (0 <= i) && (i < R[Net#b]) && (AT#Mod(i, 2) == 0) ==> (M[Net#b][i] == M[Net#d][AT#Div(i, 2)])
   );
-  assert {:msg "  25.16: Sub-actor action at 2.3 might not preserve the channel invariant"} (forall i: int :: 
-    (0 <= i) && (i < R[Net#b]) && (at$mod(i, 2) == 1) ==> (M[Net#b][i] == M[Net#c][at$div(i, 2)])
+  assert {:msg "  25.3: Sub-actor action at 3.3 might not preserve the channel invariant"} (forall i: int :: 
+    (0 <= i) && (i < R[Net#b]) && (AT#Mod(i, 2) == 1) ==> (M[Net#b][i] == M[Net#c][AT#Div(i, 2)])
   );
 }
-procedure Net#anon$3#Split#anon$1()
-  modifies C, R, M;
+procedure Net#anon$3#Split#anon$1#5()
+  modifies C, R, M, St;
 {
+  var St#next: State;
   var in#i: int;
   assume C#init[Net#a] == 2;
   assume C#init[Net#b] == 0;
   assume C#init[Net#c] == 0;
   assume C#init[Net#d] == 0;
+  assume R[Net#a] == (R[Net#b] + C[Net#b]);
   assume R[Net#d] == 0;
   assume 0 <= C[Net#d];
   assume 0 <= R[Net#d];
@@ -163,58 +176,60 @@ procedure Net#anon$3#Split#anon$1()
   assume 0 <= C[Net#a];
   assume 0 <= R[Net#a];
   assume (M[Net#a][0] < 0) && (M[Net#a][1] > 0);
-  assume (R[Net#b] + C[Net#b]) == R[Net#a];
-  assume (R[Net#d] + C[Net#d]) == at$div(R[Net#b] + 1, 2);
-  assume (R[Net#c] + C[Net#c]) == at$div(R[Net#b], 2);
+  assume (R[Net#d] + C[Net#d]) == AT#Div(R[Net#b] + 1, 2);
+  assume (R[Net#c] + C[Net#c]) == AT#Div(R[Net#b], 2);
   assume (forall i: int :: 
     (0 <= i) && (i < (R[Net#b] + C[Net#b])) ==> (M[Net#b][i] == M[Net#a][i])
   );
   assume (forall i: int :: 
-    (0 <= i) && (i < R[Net#b]) && (at$mod(i, 2) == 0) ==> (M[Net#b][i] == M[Net#d][at$div(i, 2)])
+    (0 <= i) && (i < R[Net#b]) && (AT#Mod(i, 2) == 0) ==> (M[Net#b][i] == M[Net#d][AT#Div(i, 2)])
   );
   assume (forall i: int :: 
-    (0 <= i) && (i < R[Net#b]) && (at$mod(i, 2) == 1) ==> (M[Net#b][i] == M[Net#c][at$div(i, 2)])
+    (0 <= i) && (i < R[Net#b]) && (AT#Mod(i, 2) == 1) ==> (M[Net#b][i] == M[Net#c][AT#Div(i, 2)])
   );
   assume 0 <= M[Net#b][R[Net#b] - 0];
+  assume true;
   assume (1 <= C[Net#b]) && (0 <= M[Net#b][R[Net#b] - 0]);
   in#i := M[Net#b][R[Net#b]];
   R[Net#b] := R[Net#b] + 1;
   C[Net#b] := C[Net#b] - 1;
   M[Net#c][R[Net#c] + C[Net#c]] := in#i;
   C[Net#c] := C[Net#c] + 1;
-  assert {:msg "  Sub-actor action at 6.3 might not preserve the channel invariant"} R[Net#d] == 0;
-  assert {:msg "  Sub-actor action at 6.3 might not preserve the channel invariant"} 0 <= C[Net#d];
-  assert {:msg "  Sub-actor action at 6.3 might not preserve the channel invariant"} 0 <= R[Net#d];
-  assert {:msg "  Sub-actor action at 6.3 might not preserve the channel invariant"} R[Net#c] == 0;
-  assert {:msg "  Sub-actor action at 6.3 might not preserve the channel invariant"} 0 <= C[Net#c];
-  assert {:msg "  Sub-actor action at 6.3 might not preserve the channel invariant"} 0 <= R[Net#c];
-  assert {:msg "  Sub-actor action at 6.3 might not preserve the channel invariant"} 0 <= C[Net#b];
-  assert {:msg "  Sub-actor action at 6.3 might not preserve the channel invariant"} 0 <= R[Net#b];
-  assert {:msg "  Sub-actor action at 6.3 might not preserve the channel invariant"} (R[Net#a] + C[Net#a]) == C#init[Net#a];
-  assert {:msg "  Sub-actor action at 6.3 might not preserve the channel invariant"} 0 <= C[Net#a];
-  assert {:msg "  Sub-actor action at 6.3 might not preserve the channel invariant"} 0 <= R[Net#a];
-  assert {:msg "  19.15: Sub-actor action at 6.3 might not preserve the channel invariant"} (M[Net#a][0] < 0) && (M[Net#a][1] > 0);
-  assert {:msg "  20.15: Sub-actor action at 6.3 might not preserve the channel invariant"} (R[Net#b] + C[Net#b]) == R[Net#a];
-  assert {:msg "  21.15: Sub-actor action at 6.3 might not preserve the channel invariant"} (R[Net#d] + C[Net#d]) == at$div(R[Net#b] + 1, 2);
-  assert {:msg "  22.15: Sub-actor action at 6.3 might not preserve the channel invariant"} (R[Net#c] + C[Net#c]) == at$div(R[Net#b], 2);
-  assert {:msg "  23.16: Sub-actor action at 6.3 might not preserve the channel invariant"} (forall i: int :: 
+  assert {:msg "  Sub-actor action at 7.3 might not preserve the channel invariant (generated)"} R[Net#a] == (R[Net#b] + C[Net#b]);
+  assert {:msg "  Sub-actor action at 7.3 might not preserve the channel invariant (generated)"} R[Net#d] == 0;
+  assert {:msg "  Sub-actor action at 7.3 might not preserve the channel invariant (generated)"} 0 <= C[Net#d];
+  assert {:msg "  Sub-actor action at 7.3 might not preserve the channel invariant (generated)"} 0 <= R[Net#d];
+  assert {:msg "  Sub-actor action at 7.3 might not preserve the channel invariant (generated)"} R[Net#c] == 0;
+  assert {:msg "  Sub-actor action at 7.3 might not preserve the channel invariant (generated)"} 0 <= C[Net#c];
+  assert {:msg "  Sub-actor action at 7.3 might not preserve the channel invariant (generated)"} 0 <= R[Net#c];
+  assert {:msg "  Sub-actor action at 7.3 might not preserve the channel invariant (generated)"} 0 <= C[Net#b];
+  assert {:msg "  Sub-actor action at 7.3 might not preserve the channel invariant (generated)"} 0 <= R[Net#b];
+  assert {:msg "  Sub-actor action at 7.3 might not preserve the channel invariant (generated)"} (R[Net#a] + C[Net#a]) == C#init[Net#a];
+  assert {:msg "  Sub-actor action at 7.3 might not preserve the channel invariant (generated)"} 0 <= C[Net#a];
+  assert {:msg "  Sub-actor action at 7.3 might not preserve the channel invariant (generated)"} 0 <= R[Net#a];
+  assert {:msg "  20.3: Sub-actor action at 7.3 might not preserve the channel invariant"} (M[Net#a][0] < 0) && (M[Net#a][1] > 0);
+  assert {:msg "  21.3: Sub-actor action at 7.3 might not preserve the channel invariant"} (R[Net#d] + C[Net#d]) == AT#Div(R[Net#b] + 1, 2);
+  assert {:msg "  22.3: Sub-actor action at 7.3 might not preserve the channel invariant"} (R[Net#c] + C[Net#c]) == AT#Div(R[Net#b], 2);
+  assert {:msg "  23.3: Sub-actor action at 7.3 might not preserve the channel invariant"} (forall i: int :: 
     (0 <= i) && (i < (R[Net#b] + C[Net#b])) ==> (M[Net#b][i] == M[Net#a][i])
   );
-  assert {:msg "  24.16: Sub-actor action at 6.3 might not preserve the channel invariant"} (forall i: int :: 
-    (0 <= i) && (i < R[Net#b]) && (at$mod(i, 2) == 0) ==> (M[Net#b][i] == M[Net#d][at$div(i, 2)])
+  assert {:msg "  24.3: Sub-actor action at 7.3 might not preserve the channel invariant"} (forall i: int :: 
+    (0 <= i) && (i < R[Net#b]) && (AT#Mod(i, 2) == 0) ==> (M[Net#b][i] == M[Net#d][AT#Div(i, 2)])
   );
-  assert {:msg "  25.16: Sub-actor action at 6.3 might not preserve the channel invariant"} (forall i: int :: 
-    (0 <= i) && (i < R[Net#b]) && (at$mod(i, 2) == 1) ==> (M[Net#b][i] == M[Net#c][at$div(i, 2)])
+  assert {:msg "  25.3: Sub-actor action at 7.3 might not preserve the channel invariant"} (forall i: int :: 
+    (0 <= i) && (i < R[Net#b]) && (AT#Mod(i, 2) == 1) ==> (M[Net#b][i] == M[Net#c][AT#Div(i, 2)])
   );
 }
-procedure Net#anon$3#Split#anon$2()
-  modifies C, R, M;
+procedure Net#anon$3#Split#anon$2#6()
+  modifies C, R, M, St;
 {
+  var St#next: State;
   var in#i: int;
   assume C#init[Net#a] == 2;
   assume C#init[Net#b] == 0;
   assume C#init[Net#c] == 0;
   assume C#init[Net#d] == 0;
+  assume R[Net#a] == (R[Net#b] + C[Net#b]);
   assume R[Net#d] == 0;
   assume 0 <= C[Net#d];
   assume 0 <= R[Net#d];
@@ -227,57 +242,58 @@ procedure Net#anon$3#Split#anon$2()
   assume 0 <= C[Net#a];
   assume 0 <= R[Net#a];
   assume (M[Net#a][0] < 0) && (M[Net#a][1] > 0);
-  assume (R[Net#b] + C[Net#b]) == R[Net#a];
-  assume (R[Net#d] + C[Net#d]) == at$div(R[Net#b] + 1, 2);
-  assume (R[Net#c] + C[Net#c]) == at$div(R[Net#b], 2);
+  assume (R[Net#d] + C[Net#d]) == AT#Div(R[Net#b] + 1, 2);
+  assume (R[Net#c] + C[Net#c]) == AT#Div(R[Net#b], 2);
   assume (forall i: int :: 
     (0 <= i) && (i < (R[Net#b] + C[Net#b])) ==> (M[Net#b][i] == M[Net#a][i])
   );
   assume (forall i: int :: 
-    (0 <= i) && (i < R[Net#b]) && (at$mod(i, 2) == 0) ==> (M[Net#b][i] == M[Net#d][at$div(i, 2)])
+    (0 <= i) && (i < R[Net#b]) && (AT#Mod(i, 2) == 0) ==> (M[Net#b][i] == M[Net#d][AT#Div(i, 2)])
   );
   assume (forall i: int :: 
-    (0 <= i) && (i < R[Net#b]) && (at$mod(i, 2) == 1) ==> (M[Net#b][i] == M[Net#c][at$div(i, 2)])
+    (0 <= i) && (i < R[Net#b]) && (AT#Mod(i, 2) == 1) ==> (M[Net#b][i] == M[Net#c][AT#Div(i, 2)])
   );
   assume M[Net#b][R[Net#b] - 0] < 0;
+  assume true;
   assume (1 <= C[Net#b]) && (M[Net#b][R[Net#b] - 0] < 0);
   in#i := M[Net#b][R[Net#b]];
   R[Net#b] := R[Net#b] + 1;
   C[Net#b] := C[Net#b] - 1;
   M[Net#d][R[Net#d] + C[Net#d]] := in#i;
   C[Net#d] := C[Net#d] + 1;
-  assert {:msg "  Sub-actor action at 9.3 might not preserve the channel invariant"} R[Net#d] == 0;
-  assert {:msg "  Sub-actor action at 9.3 might not preserve the channel invariant"} 0 <= C[Net#d];
-  assert {:msg "  Sub-actor action at 9.3 might not preserve the channel invariant"} 0 <= R[Net#d];
-  assert {:msg "  Sub-actor action at 9.3 might not preserve the channel invariant"} R[Net#c] == 0;
-  assert {:msg "  Sub-actor action at 9.3 might not preserve the channel invariant"} 0 <= C[Net#c];
-  assert {:msg "  Sub-actor action at 9.3 might not preserve the channel invariant"} 0 <= R[Net#c];
-  assert {:msg "  Sub-actor action at 9.3 might not preserve the channel invariant"} 0 <= C[Net#b];
-  assert {:msg "  Sub-actor action at 9.3 might not preserve the channel invariant"} 0 <= R[Net#b];
-  assert {:msg "  Sub-actor action at 9.3 might not preserve the channel invariant"} (R[Net#a] + C[Net#a]) == C#init[Net#a];
-  assert {:msg "  Sub-actor action at 9.3 might not preserve the channel invariant"} 0 <= C[Net#a];
-  assert {:msg "  Sub-actor action at 9.3 might not preserve the channel invariant"} 0 <= R[Net#a];
-  assert {:msg "  19.15: Sub-actor action at 9.3 might not preserve the channel invariant"} (M[Net#a][0] < 0) && (M[Net#a][1] > 0);
-  assert {:msg "  20.15: Sub-actor action at 9.3 might not preserve the channel invariant"} (R[Net#b] + C[Net#b]) == R[Net#a];
-  assert {:msg "  21.15: Sub-actor action at 9.3 might not preserve the channel invariant"} (R[Net#d] + C[Net#d]) == at$div(R[Net#b] + 1, 2);
-  assert {:msg "  22.15: Sub-actor action at 9.3 might not preserve the channel invariant"} (R[Net#c] + C[Net#c]) == at$div(R[Net#b], 2);
-  assert {:msg "  23.16: Sub-actor action at 9.3 might not preserve the channel invariant"} (forall i: int :: 
+  assert {:msg "  Sub-actor action at 10.3 might not preserve the channel invariant (generated)"} R[Net#a] == (R[Net#b] + C[Net#b]);
+  assert {:msg "  Sub-actor action at 10.3 might not preserve the channel invariant (generated)"} R[Net#d] == 0;
+  assert {:msg "  Sub-actor action at 10.3 might not preserve the channel invariant (generated)"} 0 <= C[Net#d];
+  assert {:msg "  Sub-actor action at 10.3 might not preserve the channel invariant (generated)"} 0 <= R[Net#d];
+  assert {:msg "  Sub-actor action at 10.3 might not preserve the channel invariant (generated)"} R[Net#c] == 0;
+  assert {:msg "  Sub-actor action at 10.3 might not preserve the channel invariant (generated)"} 0 <= C[Net#c];
+  assert {:msg "  Sub-actor action at 10.3 might not preserve the channel invariant (generated)"} 0 <= R[Net#c];
+  assert {:msg "  Sub-actor action at 10.3 might not preserve the channel invariant (generated)"} 0 <= C[Net#b];
+  assert {:msg "  Sub-actor action at 10.3 might not preserve the channel invariant (generated)"} 0 <= R[Net#b];
+  assert {:msg "  Sub-actor action at 10.3 might not preserve the channel invariant (generated)"} (R[Net#a] + C[Net#a]) == C#init[Net#a];
+  assert {:msg "  Sub-actor action at 10.3 might not preserve the channel invariant (generated)"} 0 <= C[Net#a];
+  assert {:msg "  Sub-actor action at 10.3 might not preserve the channel invariant (generated)"} 0 <= R[Net#a];
+  assert {:msg "  20.3: Sub-actor action at 10.3 might not preserve the channel invariant"} (M[Net#a][0] < 0) && (M[Net#a][1] > 0);
+  assert {:msg "  21.3: Sub-actor action at 10.3 might not preserve the channel invariant"} (R[Net#d] + C[Net#d]) == AT#Div(R[Net#b] + 1, 2);
+  assert {:msg "  22.3: Sub-actor action at 10.3 might not preserve the channel invariant"} (R[Net#c] + C[Net#c]) == AT#Div(R[Net#b], 2);
+  assert {:msg "  23.3: Sub-actor action at 10.3 might not preserve the channel invariant"} (forall i: int :: 
     (0 <= i) && (i < (R[Net#b] + C[Net#b])) ==> (M[Net#b][i] == M[Net#a][i])
   );
-  assert {:msg "  24.16: Sub-actor action at 9.3 might not preserve the channel invariant"} (forall i: int :: 
-    (0 <= i) && (i < R[Net#b]) && (at$mod(i, 2) == 0) ==> (M[Net#b][i] == M[Net#d][at$div(i, 2)])
+  assert {:msg "  24.3: Sub-actor action at 10.3 might not preserve the channel invariant"} (forall i: int :: 
+    (0 <= i) && (i < R[Net#b]) && (AT#Mod(i, 2) == 0) ==> (M[Net#b][i] == M[Net#d][AT#Div(i, 2)])
   );
-  assert {:msg "  25.16: Sub-actor action at 9.3 might not preserve the channel invariant"} (forall i: int :: 
-    (0 <= i) && (i < R[Net#b]) && (at$mod(i, 2) == 1) ==> (M[Net#b][i] == M[Net#c][at$div(i, 2)])
+  assert {:msg "  25.3: Sub-actor action at 10.3 might not preserve the channel invariant"} (forall i: int :: 
+    (0 <= i) && (i < R[Net#b]) && (AT#Mod(i, 2) == 1) ==> (M[Net#b][i] == M[Net#c][AT#Div(i, 2)])
   );
 }
-procedure Net#anon$3#exit()
-  modifies C, R, M;
+procedure Net#anon$3#exit#7()
+  modifies C, R, M, St;
 {
   assume C#init[Net#a] == 2;
   assume C#init[Net#b] == 0;
   assume C#init[Net#c] == 0;
   assume C#init[Net#d] == 0;
+  assume R[Net#a] == (R[Net#b] + C[Net#b]);
   assume R[Net#d] == 0;
   assume 0 <= C[Net#d];
   assume 0 <= R[Net#d];
@@ -290,25 +306,24 @@ procedure Net#anon$3#exit()
   assume 0 <= C[Net#a];
   assume 0 <= R[Net#a];
   assume (M[Net#a][0] < 0) && (M[Net#a][1] > 0);
-  assume (R[Net#b] + C[Net#b]) == R[Net#a];
-  assume (R[Net#d] + C[Net#d]) == at$div(R[Net#b] + 1, 2);
-  assume (R[Net#c] + C[Net#c]) == at$div(R[Net#b], 2);
+  assume (R[Net#d] + C[Net#d]) == AT#Div(R[Net#b] + 1, 2);
+  assume (R[Net#c] + C[Net#c]) == AT#Div(R[Net#b], 2);
   assume (forall i: int :: 
     (0 <= i) && (i < (R[Net#b] + C[Net#b])) ==> (M[Net#b][i] == M[Net#a][i])
   );
   assume (forall i: int :: 
-    (0 <= i) && (i < R[Net#b]) && (at$mod(i, 2) == 0) ==> (M[Net#b][i] == M[Net#d][at$div(i, 2)])
+    (0 <= i) && (i < R[Net#b]) && (AT#Mod(i, 2) == 0) ==> (M[Net#b][i] == M[Net#d][AT#Div(i, 2)])
   );
   assume (forall i: int :: 
-    (0 <= i) && (i < R[Net#b]) && (at$mod(i, 2) == 1) ==> (M[Net#b][i] == M[Net#c][at$div(i, 2)])
+    (0 <= i) && (i < R[Net#b]) && (AT#Mod(i, 2) == 1) ==> (M[Net#b][i] == M[Net#c][AT#Div(i, 2)])
   );
   assume !(((1 <= C[Net#a]) || ((1 <= C[Net#b]) && (0 <= M[Net#b][R[Net#b] - 0]))) || ((1 <= C[Net#b]) && (M[Net#b][R[Net#b] - 0] < 0)));
-  assert {:msg "  15.3: The network might leave unread tokens on channel a"} C[Net#a] == 0;
-  assert {:msg "  15.3: The network might leave unread tokens on channel b"} C[Net#b] == 0;
-  assert {:msg "  15.3: The network might not produce the specified number of tokens on output out1"} C[Net#c] == 1;
-  assert {:msg "  15.3: The network might not produce the specified number of tokens on output out2"} C[Net#d] == 1;
-  assert {:msg "  15.31: Network output might not conform to specified action output"} M[Net#c][0] == M[Net#a][1];
-  assert {:msg "  15.42: Network output might not conform to specified action output"} M[Net#d][0] == M[Net#a][0];
+  assert {:msg "  16.3: The network might leave unread tokens on channel a"} C[Net#a] == 0;
+  assert {:msg "  16.3: The network might leave unread tokens on channel b"} C[Net#b] == 0;
+  assert {:msg "  16.3: The network might not produce the specified number of tokens on output out1"} C[Net#c] == 1;
+  assert {:msg "  16.3: The network might not produce the specified number of tokens on output out2"} C[Net#d] == 1;
+  assert {:msg "  16.31: Network output might not conform to specified action output"} M[Net#c][0] == M[Net#a][1];
+  assert {:msg "  16.42: Network output might not conform to specified action output"} M[Net#d][0] == M[Net#a][0];
   R[Net#c] := R[Net#c] + C[Net#c];
   C[Net#c] := 0;
   R[Net#d] := R[Net#d] + C[Net#d];
