tests/NonDetMerge.bpl
@@ -1,0 +1,144 @@
+
+// ---------------------------------------------------------------
+// -- Types and global variables ---------------------------------
+// ---------------------------------------------------------------
+type Chan a;
+type CType = <a>[Chan a]int;
+type MType = <a>[Chan a][int]a;
+type State;
+var M: MType;
+var C: CType;
+var R: CType; 
+var C#init: CType;
+
+// ---------------------------------------------------------------
+// -- End of prelude ---------------------------------------------
+// ---------------------------------------------------------------
+
+procedure NonDetMerge#a1()
+{
+  var i: int;
+  assume true;
+}
+procedure NonDetMerge#a2()
+{
+  var i: int;
+  assume true;
+}
+const unique Top#a: Chan (int);
+const unique Top#b: Chan (int);
+const unique Top#c: Chan (int);
+procedure Top#anon$0#entry()
+  modifies C, R, M;
+{
+  assume C#init[Top#a] == 1;
+  assume C#init[Top#b] == 1;
+  assume C#init[Top#c] == 0;
+  assume R[Top#a] == 0;
+  assume R[Top#b] == 0;
+  assume R[Top#c] == 0;
+  assume C#init == C;
+  assert {:msg "  Channel invariant might not hold on action entry"} R[Top#c] == 0;
+  assert {:msg "  Channel invariant might not hold on action entry"} 0 <= C[Top#c];
+  assert {:msg "  Channel invariant might not hold on action entry"} 0 <= R[Top#c];
+  assert {:msg "  Channel invariant might not hold on action entry"} (R[Top#b] + C[Top#b]) == C#init[Top#b];
+  assert {:msg "  Channel invariant might not hold on action entry"} 0 <= C[Top#b];
+  assert {:msg "  Channel invariant might not hold on action entry"} 0 <= R[Top#b];
+  assert {:msg "  Channel invariant might not hold on action entry"} (R[Top#a] + C[Top#a]) == C#init[Top#a];
+  assert {:msg "  Channel invariant might not hold on action entry"} 0 <= C[Top#a];
+  assert {:msg "  Channel invariant might not hold on action entry"} 0 <= R[Top#a];
+  assert {:msg "  9.15: Channel invariant might not hold on action entry"} (R[Top#c] + C[Top#c]) == (R[Top#a] + R[Top#b]);
+}
+procedure Top#anon$0#NonDetMerge#a1()
+  modifies C, R, M;
+{
+  var x1#i: int;
+  assume C#init[Top#a] == 1;
+  assume C#init[Top#b] == 1;
+  assume C#init[Top#c] == 0;
+  assume R[Top#c] == 0;
+  assume 0 <= C[Top#c];
+  assume 0 <= R[Top#c];
+  assume (R[Top#b] + C[Top#b]) == C#init[Top#b];
+  assume 0 <= C[Top#b];
+  assume 0 <= R[Top#b];
+  assume (R[Top#a] + C[Top#a]) == C#init[Top#a];
+  assume 0 <= C[Top#a];
+  assume 0 <= R[Top#a];
+  assume (R[Top#c] + C[Top#c]) == (R[Top#a] + R[Top#b]);
+  assume 1 <= C[Top#a];
+  x1#i := M[Top#a][R[Top#a]];
+  R[Top#a] := R[Top#a] + 1;
+  C[Top#a] := C[Top#a] - 1;
+  M[Top#c][R[Top#c] + C[Top#c]] := x1#i;
+  C[Top#c] := C[Top#c] + 1;
+  assert {:msg "  Sub-actor action at 2.3 might not preserve the channel invariant"} R[Top#c] == 0;
+  assert {:msg "  Sub-actor action at 2.3 might not preserve the channel invariant"} 0 <= C[Top#c];
+  assert {:msg "  Sub-actor action at 2.3 might not preserve the channel invariant"} 0 <= R[Top#c];
+  assert {:msg "  Sub-actor action at 2.3 might not preserve the channel invariant"} (R[Top#b] + C[Top#b]) == C#init[Top#b];
+  assert {:msg "  Sub-actor action at 2.3 might not preserve the channel invariant"} 0 <= C[Top#b];
+  assert {:msg "  Sub-actor action at 2.3 might not preserve the channel invariant"} 0 <= R[Top#b];
+  assert {:msg "  Sub-actor action at 2.3 might not preserve the channel invariant"} (R[Top#a] + C[Top#a]) == C#init[Top#a];
+  assert {:msg "  Sub-actor action at 2.3 might not preserve the channel invariant"} 0 <= C[Top#a];
+  assert {:msg "  Sub-actor action at 2.3 might not preserve the channel invariant"} 0 <= R[Top#a];
+  assert {:msg "  9.15: Sub-actor action at 2.3 might not preserve the channel invariant"} (R[Top#c] + C[Top#c]) == (R[Top#a] + R[Top#b]);
+}
+procedure Top#anon$0#NonDetMerge#a2()
+  modifies C, R, M;
+{
+  var x2#i: int;
+  assume C#init[Top#a] == 1;
+  assume C#init[Top#b] == 1;
+  assume C#init[Top#c] == 0;
+  assume R[Top#c] == 0;
+  assume 0 <= C[Top#c];
+  assume 0 <= R[Top#c];
+  assume (R[Top#b] + C[Top#b]) == C#init[Top#b];
+  assume 0 <= C[Top#b];
+  assume 0 <= R[Top#b];
+  assume (R[Top#a] + C[Top#a]) == C#init[Top#a];
+  assume 0 <= C[Top#a];
+  assume 0 <= R[Top#a];
+  assume (R[Top#c] + C[Top#c]) == (R[Top#a] + R[Top#b]);
+  assume 1 <= C[Top#b];
+  x2#i := M[Top#b][R[Top#b]];
+  R[Top#b] := R[Top#b] + 1;
+  C[Top#b] := C[Top#b] - 1;
+  M[Top#c][R[Top#c] + C[Top#c]] := x2#i;
+  C[Top#c] := C[Top#c] + 1;
+  assert {:msg "  Sub-actor action at 3.3 might not preserve the channel invariant"} R[Top#c] == 0;
+  assert {:msg "  Sub-actor action at 3.3 might not preserve the channel invariant"} 0 <= C[Top#c];
+  assert {:msg "  Sub-actor action at 3.3 might not preserve the channel invariant"} 0 <= R[Top#c];
+  assert {:msg "  Sub-actor action at 3.3 might not preserve the channel invariant"} (R[Top#b] + C[Top#b]) == C#init[Top#b];
+  assert {:msg "  Sub-actor action at 3.3 might not preserve the channel invariant"} 0 <= C[Top#b];
+  assert {:msg "  Sub-actor action at 3.3 might not preserve the channel invariant"} 0 <= R[Top#b];
+  assert {:msg "  Sub-actor action at 3.3 might not preserve the channel invariant"} (R[Top#a] + C[Top#a]) == C#init[Top#a];
+  assert {:msg "  Sub-actor action at 3.3 might not preserve the channel invariant"} 0 <= C[Top#a];
+  assert {:msg "  Sub-actor action at 3.3 might not preserve the channel invariant"} 0 <= R[Top#a];
+  assert {:msg "  9.15: Sub-actor action at 3.3 might not preserve the channel invariant"} (R[Top#c] + C[Top#c]) == (R[Top#a] + R[Top#b]);
+}
+procedure Top#anon$0#exit()
+  modifies C, R, M;
+{
+  assume C#init[Top#a] == 1;
+  assume C#init[Top#b] == 1;
+  assume C#init[Top#c] == 0;
+  assume R[Top#c] == 0;
+  assume 0 <= C[Top#c];
+  assume 0 <= R[Top#c];
+  assume (R[Top#b] + C[Top#b]) == C#init[Top#b];
+  assume 0 <= C[Top#b];
+  assume 0 <= R[Top#b];
+  assume (R[Top#a] + C[Top#a]) == C#init[Top#a];
+  assume 0 <= C[Top#a];
+  assume 0 <= R[Top#a];
+  assume (R[Top#c] + C[Top#c]) == (R[Top#a] + R[Top#b]);
+  assume !((1 <= C[Top#a]) || (1 <= C[Top#b]));
+  assert {:msg "  7.3: The network might leave unread tokens on channel a"} C[Top#a] == 0;
+  assert {:msg "  7.3: The network might leave unread tokens on channel b"} C[Top#b] == 0;
+  assert {:msg "  7.3: The network might not produce the specified number of tokens on output out"} C[Top#c] == 2;
+  assert {:msg "  7.36: Network output might not conform to specified action output"} M[Top#c][0] == M[Top#a][0];
+  assert {:msg "  7.38: Network output might not conform to specified action output"} M[Top#c][1] == M[Top#b][0];
+  R[Top#c] := R[Top#c] + C[Top#c];
+  C[Top#c] := 0;
+}
